kernel/sorts.mli
@@ -203,6 +203,7 @@ val relevance_equal : relevance -> relevance -> bool
 val relevance_subst_fn : (QVar.t -> Quality.t) -> relevance -> relevance
 
 val relevance_of_sort : t -> relevance
+val relevance_of_quality : Quality.t -> relevance
 val relevance_of_sort_family : family -> relevance
 
 val debug_print : t -> Pp.t
